Created branch dep_debruijn to try changing the undependent deBruijn indices to be dependent

Complexity.v
@@ -1,11 +1,9 @@
+Require Import Arith.
+Require Import List.
 Require Import Util.
 Require Import NonnegRational.
 
 Export NonnegRational.
-
-Notation var := nat (only parsing).
-Notation Vbound n := (n : nat).
-Notation "# n" := (Vbound n) (at level 3).
 
 (* 
   There are two statistics (or 'sizes', 'size measures') for each value :
@@ -26,81 +24,150 @@ Inductive path_command :=
 .
 
 Notation path := (list path_command). (* The query path into a inner-component *)
-Definition var_path := (var * path)%type.
 
-(* complexity expression *)
-Inductive cexpr :=
-(* it is a ring *)
-| F0
-| Fadd (a b : cexpr)
-| F1
-| Fmul (a b : cexpr)
-(* it is a module, so also an algebra*)
-| Fscale (_ : QN) (_ : cexpr)
-(* some special operations *)
-| Fmax (a b : cexpr)
-| Flog (base : QN) (n : cexpr)
-| Fexp (base : QN) (n : cexpr)
-(* variables *)
-| Fvar (x : var_path) (stat : stat_idx)
-(* minus 1 (lower-capped by 0) *)
-| Fminus1 (_ : cexpr)
+Inductive CtxEntry :=
+| CEtype
+| CEexpr
 .
 
-Instance Max_cexpr : Max cexpr :=
+Definition context := list CtxEntry.
+
+Class Leb A B :=
   {
-    max := Fmax
+    leb : A -> B -> bool
   }.
 
-Definition Fconst c := Fscale c F1.
-Coercion Fconst : QN >-> cexpr.
+Infix "<=?" := leb (at level 70).
+Notation "a <? b" := (negb (b <=? a)) (at level 70).
 
-Definition stats := (cexpr * cexpr)%type.
+Global Instance Leb_nat : Leb nat nat :=
+  {
+    leb := Compare_dec.leb
+  }.
 
-Definition stats_get (idx : stat_idx) (ss : stats) := 
-  match ss with
-    | (n0, n1) =>
-      match idx with
-        | O => n0
-        | _ => n1
+Definition boolProp b := b = true.
+Coercion boolProp : bool >-> Sortclass.
+
+Inductive ordinal n :=
+| Ordinal m (_ : m <? n)
+.
+
+Notation "''I_' n" := (ordinal n) (at level 8, n at level 2, format "''I_' n").
+Notation "# n" := (Ordinal _ n (eq_refl true)) (at level 3).
+
+Program Fixpoint nthI {A} (ls : list A) (i : 'I_(length ls)) :=
+  match ls with
+    | x :: xs =>
+      match i with
+        | Ordinal 0 _ => x
+        | Ordinal (S n) _ => nthI xs #n
       end
+    | nil => _
   end.
+Next Obligation.
+  destruct i; simpl in *; intuition.
+Defined.
 
-Inductive size :=
-| Svar (x : var_path)
-| Sstats (_ : stats)
-| Sinlinr (a b: size)
-| Spair (a b: size)
-| Sfold (_ : size)
-| Shide (_ : size)
-.
+Goal nthI (1 :: 2 :: nil) (Ordinal 2 1 eq_refl) = 2. eauto. Qed.
 
-Definition stats_binop {A} (f : cexpr -> cexpr -> A) (a b : stats) :=
-  match a, b with
-    | (a0, a1), (b0, b1) => (f a0 b0, f a1 b1)
-  end.
+Section ctx.
 
-Definition stats_add := stats_binop Fadd.
-Infix "+" := stats_add : stats_scope.
-Delimit Scope stats_scope with stats.
-Definition stats_max := stats_binop Fmax.
-Instance Max_stats : Max stats :=
-  {
-    max := stats_max
-  }.
+  Variable ctx : context.
+  
+  Inductive var : CtxEntry -> Type :=
+  | Var (i : 'I_(length ctx)) : var (nthI ctx i)
+  .
 
-Definition zeros : stats := (F0, F0).
+  Definition var_path := (var CEexpr * path)%type.
 
-Fixpoint summarize (s : size) : stats :=
-  match s with
-    | Svar x => (Fvar x 0%nat, Fvar x 1%nat)
-    | Sstats ss => ss
-    | Spair a b => 
-      (summarize a + summarize b)%stats
-    | Sinlinr a b => 
-      max (summarize a) (summarize b)
-    | Sfold s =>
-      ((F1, F1) + summarize s)%stats
-    | Shide s => zeros
-  end.
+  (* complexity expression *)
+  Inductive cexpr :=
+  (* it is a ring *)
+  | F0
+  | Fadd (a b : cexpr)
+  | F1
+  | Fmul (a b : cexpr)
+  (* it is a module, so also an algebra*)
+  | Fscale (_ : QN) (_ : cexpr)
+  (* some special operations *)
+  | Fmax (a b : cexpr)
+  | Flog (base : QN) (n : cexpr)
+  | Fexp (base : QN) (n : cexpr)
+  (* variables *)
+  | Fvar (x : var_path) (stat : stat_idx)
+  (* minus 1 (lower-capped by 0) *)
+  | Fminus1 (_ : cexpr)
+  .
+
+  Global Instance Max_cexpr : Max cexpr :=
+    {
+      max := Fmax
+    }.
+
+  (* Definition Fconst c := Fscale c F1. *)
+  (* Coercion Fconst : QN >-> cexpr. *)
+
+  Definition stats := (cexpr * cexpr)%type.
+
+  Definition stats_get (idx : stat_idx) (ss : stats) := 
+    match ss with
+      | (n0, n1) =>
+        match idx with
+          | O => n0
+          | _ => n1
+        end
+    end.
+
+  Inductive size :=
+  | Svar (x : var_path)
+  | Sstats (_ : stats)
+  | Sinlinr (a b: size)
+  | Spair (a b: size)
+  | Sfold (_ : size)
+  | Shide (_ : size)
+  .
+
+  Definition stats_binop {A} (f : cexpr -> cexpr -> A) (a b : stats) :=
+    match a, b with
+      | (a0, a1), (b0, b1) => (f a0 b0, f a1 b1)
+    end.
+
+  Definition stats_add := stats_binop Fadd.
+  Infix "+" := stats_add : stats_scope.
+  Delimit Scope stats_scope with stats.
+  Definition stats_max := stats_binop Fmax.
+  Global Instance Max_stats : Max stats :=
+    {
+      max := stats_max
+    }.
+
+  Definition zeros : stats := (F0, F0).
+
+  Fixpoint summarize (s : size) : stats :=
+    match s with
+      | Svar x => (Fvar x 0%nat, Fvar x 1%nat)
+      | Sstats ss => ss
+      | Spair a b => 
+        (summarize a + summarize b)%stats
+      | Sinlinr a b => 
+        max (summarize a) (summarize b)
+      | Sfold s =>
+        ((F1, F1) + summarize s)%stats
+      | Shide s => zeros
+    end.
+
+End ctx.
+
+Global Arguments Fscale {ctx} _ _ .
+Global Arguments Fadd {ctx} _ _ .
+Global Arguments Fmul {ctx} _ _ .
+Global Arguments F0 {ctx} .
+Global Arguments F1 {ctx} .
+Global Arguments Flog {ctx} _ _.
+Global Arguments Fmax {ctx} _ _ .
+Global Arguments Fexp {ctx} _ _ .
+Global Arguments Fvar {ctx} _ _ .
+Global Arguments Fminus1 {ctx} _ .
+Global Arguments stats_get {ctx} _ _ .
+Global Arguments summarize {ctx} _ .
 
